updates

Veritas.Verifier.EAC.fst
@@ -28,6 +28,56 @@ let time_seq_ext (#n:nat) (itsl: its_log n): (le:vlog_ext{project_seq itsl = to_
 type eac_ts_log (#n:nat) = itsl: its_log n {is_eac_log (time_seq_ext itsl)}
 type non_eac_ts_log (#n:nat) = itsl: its_log n {not (is_eac_log (time_seq_ext itsl))}
 
+let eac_invalidating_key (#n:nat) (itsl: non_eac_ts_log #n): key =
+  let tsle = time_seq_ext itsl in
+
+  (* maximum eac valid prefix *)
+  let i = max_eac_prefix tsle in
+
+  (* ee is the entry causing eac invalidation *)
+  let ee = index tsle i in
+  
+  (* the key causing the invalidation *)
+  partn_fn eac_sm ee
+
+
+let last_valid_eac_state (#n:nat) (itsl: non_eac_ts_log #n): eac_state = 
+
+  let tsle = time_seq_ext itsl in
+  
+  let i = max_eac_prefix tsle in
+
+  (* maximum eac prefix *)
+  let tslei = prefix tsle i in
+
+  (* minimum non-eac prefix *)
+  let tslei' = prefix tsle (i + 1) in
+
+  lemma_first_invalid_key eac_sm tsle;
+
+  (* ee is the entry causing eac invalidation *)
+  let ee = index tsle i in
+  
+  (* the key causing the invalidation *)
+  let k = eac_invalidating_key itsl in
+
+  (* log entries of only key k *)
+  let tslek = partn eac_sm k tsle in
+
+  (* j the index in tslek causing invalidation *)
+  let j = max_valid_prefix eac_smk tslek in
+  //assert(filter_index_inv_map (iskey vlog_entry_key k) tsle i = j);  
+  //assert(vlog_entry_key ee = k);
+  //assert(index tslek j = ee);
+
+  let tslekj = prefix tslek j in
+  assert(valid eac_smk tslekj);
+  
+  let st = seq_machine_run eac_smk tslekj in
+  assert(st <> EACFail);
+
+  st
+
 let lemma_non_eac_time_seq_implies_hash_collision (#n:nat) (itsl: non_eac_ts_log #n): hash_collision_gen = 
   let tsl = project_seq itsl in
   let tsle = time_seq_ext itsl in
@@ -41,15 +91,34 @@ let lemma_non_eac_time_seq_implies_hash_collision (#n:nat) (itsl: non_eac_ts_log
   let tslei' = prefix tsle (i + 1) in
 
   lemma_first_invalid_key eac_sm tsle;
+
+  (* ee is the entry causing eac invalidation *)
   let ee = index tsle i in
-  let k:key = partn_fn eac_sm ee in
-  let tslek = partn eac_sm k tsle in
-  let j = max_valid_prefix eac_smk tslek in
-
-  assert(filter_index_inv_map (iskey vlog_entry_key k) tsle i = j);  
-  assert(vlog_entry_key ee = k);
-  assert(index tslek j = ee);
-
-  //let st = seq_machine_run eac_smk 
   
-  admit()
+  (* the key causing the invalidation *)
+  let k = eac_invalidating_key itsl in
+
+  (* log entries of only key k *)
+  let tslek = partn eac_sm k tsle in
+
+  (* j the index in tslek causing invalidation *)
+  let j = max_valid_prefix eac_smk tslek in
+  //assert(filter_index_inv_map (iskey vlog_entry_key k) tsle i = j);  
+  //assert(vlog_entry_key ee = k);
+  //assert(index tslek j = ee);
+
+  let tslekj = prefix tslek j in
+  assert(valid eac_smk tslekj);
+  
+  let st = seq_machine_run eac_smk tslekj in
+  assert(st <> EACFail);
+  assert(st = last_valid_eac_state itsl);
+  
+  lemma_reduce_prefix EACInit eac_add (prefix tslek (j + 1)) j;  
+  lemma_reduce_singleton st eac_add (suffix (prefix tslek (j + 1)) 1);
+  assert(eac_add ee st = EACFail);
+  
+  match st with
+  | EACInit -> admit()
+  | EACInCache m v -> admit()
+  | EACEvicted m v -> admit()
